checkpoint

examples/algorithms/qsort_arr.fst
@@ -62,19 +62,17 @@ let rec sort f i j x =
     let pivot = partition f i j i (j - 1) x in
     let h1 = ST.get () in
     sort f i pivot x;
-    (* let h2 = ST.get () in  *)
+    let h2 = ST.get () in
     sort f (pivot + 1) j x;
-    admit ()
-
-    (* let h3 = ST.get () in  *)
-    (* assert (sel h1 x = splice (sel h0 x) i (sel h1 x) j); *)
-    (* assert (sorted f (slice (sel h2 x) i pivot)); *)
-    (* assert (sorted f (slice (sel h3 x) (pivot + 1) j)); *)
+    let h3 = ST.get () in
+    assert (sel h1 x = splice (sel h0 x) i (sel h1 x) j);
+    assert (sorted f (slice (sel h2 x) i pivot));
+    assert (sorted f (slice (sel h3 x) (pivot + 1) j));
     (* assert (Eq (slice (sel h3 x) i j) *)
     (*            (append (slice (sel h2 x) i pivot) *)
     (*                    (cons (index (sel h1 x) pivot) *)
     (*                          (slice (sel h3 x) (pivot + 1) j)))); *)
-    (* admit () *)
+    admit ()
        
 
 (* val qsort: a:Type -> f:(a -> a -> Tot bool){total_order a f} -> x:array a -> ST unit  *)
